theories/examples/malloc.v
@@ -22,7 +22,7 @@ Section SimpleMalloc.
           `{MP: MachineParameters}.
 
   Definition malloc_subroutine_instrs' (offset: Z) :=
-    encodeInstrsW [
+    encodeInstrsLW [
      Lt r_t3 0 r_t1;
      Mov r_t2 PC;
      Lea r_t2 4;
@@ -56,35 +56,35 @@ Section SimpleMalloc.
   Definition malloc_subroutine_instrs :=
     malloc_subroutine_instrs' (malloc_subroutine_instrs_length - 5).
 
-  Definition malloc_inv (b e : Addr) : iProp Σ :=
+  Definition malloc_inv (b e : Addr) (v : Version) : iProp Σ :=
     (∃ b_m a_m,
-       codefrag b malloc_subroutine_instrs
+       codefrag b v malloc_subroutine_instrs
      ∗ ⌜(b + malloc_subroutine_instrs_length)%a = Some b_m⌝
-     ∗ b_m ↦ₐ (WCap RWX b_m e a_m)
-     ∗ [[a_m, e]] ↦ₐ [[ region_addrs_zeroes a_m e ]]
+     ∗ (b_m, v) ↦ₐ (LCap RWX b_m e a_m v)
+     ∗ [[a_m, e]] ↦ₐ{v} [[ region_addrs_zeroesL a_m e v ]]
      ∗ ⌜(b_m < a_m)%a ∧ (a_m <= e)%a⌝)%I.
 
-  Lemma simple_malloc_subroutine_spec (wsize: Word) (cont: Word) b e rmap N E φ :
+  Lemma simple_malloc_subroutine_spec (wsize: LWord) (cont: LWord) b e v rmap N E φ :
     dom rmap = all_registers_s ∖ {[ PC; r_t0; r_t1 ]} →
     ↑N ⊆ E →
-    (  na_inv logrel_nais N (malloc_inv b e)
+    (  na_inv logrel_nais N (malloc_inv b e v)
      ∗ na_own logrel_nais E
      ∗ ([∗ map] r↦w ∈ rmap, r ↦ᵣ w)
      ∗ r_t0 ↦ᵣ cont
-     ∗ PC ↦ᵣ WCap RX b e b
+     ∗ PC ↦ᵣ LCap RX b e b v
      ∗ r_t1 ↦ᵣ wsize
      ∗ ▷ ((na_own logrel_nais E
-          ∗ [∗ map] r↦w ∈ <[r_t2 := WInt 0%Z]>
-                         (<[r_t3 := WInt 0%Z]>
-                         (<[r_t4 := WInt 0%Z]>
+          ∗ [∗ map] r↦w ∈ <[r_t2 := LInt 0%Z]>
+                         (<[r_t3 := LInt 0%Z]>
+                         (<[r_t4 := LInt 0%Z]>
                           rmap)), r ↦ᵣ w)
           ∗ r_t0 ↦ᵣ cont
-          ∗ PC ↦ᵣ updatePcPerm cont
+          ∗ PC ↦ᵣ updatePcPermL cont
           ∗ (∃ (ba ea : Addr) size,
-            ⌜wsize = WInt size⌝
+            ⌜wsize = LWInt size⌝
             ∗ ⌜(ba + size)%a = Some ea⌝
-            ∗ r_t1 ↦ᵣ WCap RWX ba ea ba
-            ∗ [[ba, ea]] ↦ₐ [[region_addrs_zeroes ba ea]])
+            ∗ r_t1 ↦ᵣ LCap RWX ba ea ba v
+            ∗ [[ba, ea]] ↦ₐ{v} [[region_addrs_zeroesL ba ea v]])
           -∗ WP Seq (Instr Executable) {{ φ }}))
     ⊢ WP Seq (Instr Executable) {{ λ v, φ v ∨ ⌜v = FailedV⌝ }}%I.
   Proof.
@@ -112,7 +112,7 @@ Section SimpleMalloc.
     unfold malloc_subroutine_instrs_length in Hbm.
     assert (SubBounds b e b (b ^+ length malloc_subroutine_instrs)%a) by solve_addr.
     destruct wsize as [size | [ | ] | ].
-    2,3,4: iInstr "Hprog"; wp_end; eauto.
+    2,3,4: iInstr "Hprog"; try wp_end; eauto.
     do 3 iInstr "Hprog".
 
     (* we need to destruct on the cases for the size *)
@@ -133,7 +133,7 @@ Section SimpleMalloc.
     destruct (a_m + size)%a as [a_m'|] eqn:Ha_m'; cycle 1.
     { (* Failure case: no registered rule for that yet; do it the manual way *)
       iInstr_lookup "Hprog" as "Hi" "Hcont".
-      iAssert ([∗ map] k↦x ∈ (∅:gmap RegName Word), k ↦ᵣ x)%I as "-#Hregs".
+      iAssert ([∗ map] k↦x ∈ (∅:gmap RegName LWord), k ↦ᵣ x)%I as "-#Hregs".
         by rewrite big_sepM_empty.
       iDestruct (big_sepM_insert with "[$Hregs $HPC]") as "-#Hregs".
         by apply lookup_empty.
@@ -157,7 +157,7 @@ Section SimpleMalloc.
     destruct (isWithin a_m a_m' b_m e) eqn:Ha_m'_within; cycle 1.
     { (* Failure case: manual mode. *)
       iInstr_lookup "Hprog" as "Hi" "Hcont".
-      iAssert ([∗ map] k↦x ∈ (∅:gmap RegName Word), k ↦ᵣ x)%I as "-#Hregs".
+      iAssert ([∗ map] k↦x ∈ (∅:gmap RegName LWord), k ↦ᵣ x)%I as "-#Hregs".
         by rewrite big_sepM_empty.
       iDestruct (big_sepM_insert with "[$Hregs $HPC]") as "-#Hregs".
         by apply lookup_empty.
@@ -183,7 +183,7 @@ Section SimpleMalloc.
     iInstr "Hprog". solve_pure_addr.
     iGo "Hprog".
     (* continuation *)
-    rewrite (region_addrs_zeroes_split _ a_m') //; [| solve_addr].
+    rewrite (region_addrs_zeroesL_split _ a_m') //; [| solve_addr].
     iDestruct (region_mapsto_split _ _ a_m' with "Hmem") as "[Hmem_fresh Hmem]".
     solve_addr. by rewrite replicate_length //.
     iDestruct ("Hinv_close" with "[Hprog Hmemptr Hmem $Hna]") as ">Hna".
@@ -206,9 +206,9 @@ Section SimpleMalloc.
     { auto. }
   Qed.
 
-  Lemma simple_malloc_subroutine_valid N b e :
-    na_inv logrel_nais N (malloc_inv b e) -∗
-    interp (WCap E b e b).
+  Lemma simple_malloc_subroutine_valid N b e v :
+    na_inv logrel_nais N (malloc_inv b e v) -∗
+    interp (LCap E b e b v).
   Proof.
     iIntros "#Hmalloc".
     rewrite fixpoint_interp1_eq /=. iIntros (r). iNext. iModIntro.
@@ -220,14 +220,14 @@ Section SimpleMalloc.
     iDestruct (big_sepM_delete _ _ r_t1 with "Hregs") as "[r_t1 Hregs]";[rewrite !lookup_delete_ne// !lookup_insert_ne//;eauto|].
     iApply (wp_wand with "[-]").
     iApply (simple_malloc_subroutine_spec with "[- $Hown $Hmalloc $Hregs $r_t0 $HPC $r_t1]");[|solve_ndisj|].
-    3: { iSimpl. iIntros (v) "[H | ->]". iExact "H". iIntros (Hcontr); done. }
+    3: { iSimpl. iIntros (w) "[H | ->]". iExact "H". iIntros (Hcontr); done. }
     { rewrite !dom_delete_L dom_insert_L. apply regmap_full_dom in H as <-. set_solver. }
     unshelve iDestruct ("Hregs_valid" $! r_t0 _ _ H0) as "Hr0_valid";auto.
     iDestruct (jmp_to_unknown with "Hr0_valid") as "Hcont".
     iNext. iIntros "((Hown & Hregs) & Hr_t0 & HPC & Hres)".
     iDestruct "Hres" as (ba ea size Hsizeq Hsize) "[Hr_t1 Hbe]".
 
-    iMod (region_integers_alloc _ _ _ _ _ RWX with "Hbe") as "#Hbe"; auto.
+    iMod (region_integers_alloc _ _ _ _ _ _ RWX with "Hbe") as "#Hbe"; auto.
     by apply Forall_replicate.
     rewrite -!(delete_insert_ne _ r_t1)//.
     iDestruct (big_sepM_insert with "[$Hregs $Hr_t1]") as "Hregs";[apply lookup_delete|rewrite insert_delete_insert].
